src/Consensus.Tests/SignedWitnessTests.fs
@@ -1,0 +1,161 @@
+module Consensus.Tests.SignedWitnessTests
+
+open NUnit.Framework
+open FsUnit
+open Consensus
+open Consensus.Types
+open Consensus.TransactionValidation
+open Consensus.Tests.Helper
+open Wallet
+open Infrastructure
+open TestsInfrastructure.Constraints
+
+
+let chain = Chain.getChainParameters Chain.Local
+let contractPath = "./test"
+
+let code = """
+open Zen.Types
+open Zen.Base
+open Zen.Cost
+open Zen.Asset
+
+module RT = Zen.ResultT
+module Tx = Zen.TxSkeleton
+
+val main: txSkeleton -> hash -> string -> sender -> option data -> wallet -> result (txSkeleton ** option message) `cost` (64 + (64 + 64 + 0) + 19)
+let main txSkeleton contractHash command sender data wallet =
+    match sender with
+    | PK _ ->
+        let! contractAsset = getDefault contractHash in
+
+        let! txSkeleton =
+            Tx.mint 1UL contractAsset txSkeleton
+            >>=Tx.lockToContract contractAsset 1UL contractHash in
+
+        RT.ok (txSkeleton, None)
+    | _ -> RT.autoFailw "expected pk"
+
+val cf: txSkeleton -> string -> sender -> option data -> wallet -> cost nat 9
+let cf _ _ _ _ _ = ret (64 + (64 + 64 + 0) + 19)
+"""
+
+let cHash = Contract.computeHash code
+let account = createTestAccount ()
+
+let mutable acs = ActiveContractSet.empty
+
+[<OneTimeSetUp>]
+let setup () =
+    let hints = Contract.recordHints code |> Result.get
+    let contractActivation =
+        {
+            code=code;
+            hints=hints;
+            rlimit = Account.rlimit;
+            queries = ZFStar.totalQueries hints |> Result.get
+        }
+    let contract = Contract.compile contractPath contractActivation 100ul |> Result.get
+
+    acs <- ActiveContractSet.add cHash contract ActiveContractSet.empty
+
+[<Test>]
+let ``contract witness with valid signature``() =
+    let spend = {asset=cHash,Hash.zero;amount=1UL}
+    let tx =
+        {
+            inputs=[Mint spend]
+            outputs=[{lock=Contract cHash;spend=spend}]
+            witnesses=[]
+            contract=None
+        }
+
+    let txHash = Transaction.hash tx
+
+    let publicKey = ExtendedKey.getPublicKey (snd account) |> Result.get
+    let signature = ExtendedKey.sign txHash (snd account) |> Result.get
+
+    let contractWintess = ContractWitness {
+                                              cHash=cHash;
+                                              command="";
+                                              data=None;
+                                              beginInputs = 0ul;
+                                              beginOutputs = 0ul;
+                                              inputsLength=1ul;
+                                              outputsLength=1ul;
+                                              signature=Some (publicKey,signature)
+                                              cost = 211ul
+                                          }
+    let tx = {tx with witnesses= [contractWintess]}
+
+    let result = TransactionValidation.validateInContext chain (fun _ -> UtxoSet.NoOutput) contractPath 2ul acs UtxoSet.asDatabase txHash tx
+
+    result |> should be ok
+
+[<Test>]
+let ``contract witness with invalid publickey``() =
+    let spend = {asset=cHash,Hash.zero;amount=1UL}
+    let tx =
+        {
+            inputs=[Mint spend]
+            outputs=[{lock=Contract cHash;spend=spend}]
+            witnesses=[]
+            contract=None
+        }
+
+    let txHash = Transaction.hash tx
+
+    let publicKey = ExtendedKey.derivePath "m/0'" (snd account) |> Result.get |> ExtendedKey.getPublicKey |> Result.get
+    let signature = ExtendedKey.sign txHash (snd account) |> Result.get
+
+    let contractWintess = ContractWitness {
+                                              cHash=cHash;
+                                              command="";
+                                              data=None;
+                                              beginInputs = 0ul;
+                                              beginOutputs = 0ul;
+                                              inputsLength=1ul;
+                                              outputsLength=1ul;
+                                              signature=Some (publicKey,signature)
+                                              cost = 211ul
+                                          }
+    let tx = {tx with witnesses= [contractWintess]}
+
+    let result = TransactionValidation.validateInContext chain (fun _ -> UtxoSet.NoOutput) contractPath 2ul acs UtxoSet.asDatabase txHash tx
+
+    let expected:Result<Transaction*ActiveContractSet.T,ValidationError> = Error (General "invalid contract witness signature")
+
+    result |> should equal expected
+
+[<Test>]
+let ``contract witness with no signature``() =
+    let spend = {asset=cHash,Hash.zero;amount=1UL}
+    let tx =
+        {
+            inputs=[Mint spend]
+            outputs=[{lock=Contract cHash;spend=spend}]
+            witnesses=[]
+            contract=None
+        }
+
+    let txHash = Transaction.hash tx
+
+
+    let contractWintess = ContractWitness {
+                                              cHash=cHash;
+                                              command="";
+                                              data=None;
+                                              beginInputs = 0ul;
+                                              beginOutputs = 0ul;
+                                              inputsLength=1ul;
+                                              outputsLength=1ul;
+                                              signature=None
+                                              cost = 211ul
+                                          }
+    let tx = {tx with witnesses= [contractWintess]}
+
+    let result = TransactionValidation.validateInContext chain (fun _ -> UtxoSet.NoOutput) contractPath 2ul acs UtxoSet.asDatabase txHash tx
+
+    let expected:Result<Transaction*ActiveContractSet.T,ValidationError> = Error (General "expected pk")
+
+    result |> should equal expected
