src/Consensus/Crypto.fs
@@ -221,7 +221,7 @@ let sign (SecretKey secretKey) (Hash hash) =
     | Native.Result.Ok -> Signature.Signature signature
     | x -> failwithf "failed to sign %A" x
 
-let verify (PublicKey publicKey) (Signature signature) msg =
+let verify (PublicKey publicKey) (Signature signature) (Hash msg) =
     match Native.secp256k1_ecdsa_verify (context, signature, msg, publicKey) with
     | Native.Result.Ok -> Valid
     | _ -> Invalid
