src/Messaging/Services.fs
@@ -38,7 +38,7 @@ module Blockchain =
         | HandleHeaders of peerId:byte[] * BlockHeader list
 
     type Request =
-        | ExecuteContract of Hash * string * data option * TxSkeleton.T
+        | ExecuteContract of Hash * string * Crypto.PublicKey option * data option * TxSkeleton.T
         | GetBlockTemplate of pkHash:Hash
         | GetTip
         | GetBlock of Hash
@@ -61,8 +61,8 @@ module Blockchain =
     let handleMemPool client peerId txHashes =
         Command.send client serviceName (HandleMemPool (peerId,txHashes))
 
-    let executeContract client cHash command data txSkeleton =
-        ExecuteContract (cHash,command, data, txSkeleton)
+    let executeContract client cHash command sender data txSkeleton =
+        ExecuteContract (cHash,command, sender, data, txSkeleton)
         |> Request.send<Request, Result<Transaction,string>> client serviceName
 
     let validateBlock client block =
@@ -157,7 +157,7 @@ module Wallet =
         | ImportSeed of string list * byte[]
         | Spend of Hash * Spend
         | ActivateContract of string*uint32
-        | ExecuteContract of Hash * string * data option * provideReturnAddress:bool * Map<Asset, uint64>
+        | ExecuteContract of Hash * string * data option * provideReturnAddress:bool * sign:string option * Map<Asset, uint64>
         | AccountExists
         | AccountLocked
         | Unlock of byte[]
@@ -182,8 +182,8 @@ module Wallet =
     let activateContract client code numberOfBlocks =
         send<ActivateContractResponse> client serviceName (ActivateContract (code,numberOfBlocks))
 
-    let executeContract client address command data provideReturnAddress spends  =
-        send<Transaction> client serviceName (ExecuteContract (address,command,data,provideReturnAddress, spends))
+    let executeContract client address command data provideReturnAddress sign spends  =
+        send<Transaction> client serviceName (ExecuteContract (address,command,data,provideReturnAddress,sign,spends))
 
     let importSeed client words key =
         send<unit> client serviceName (ImportSeed (words, key))
