src/Node/Program.fs
@@ -162,7 +162,21 @@ let main argv =
     printfn "running..."
 
     if chain = Chain.Local then
-        let block = Block.createGenesis chainParams [Transaction.rootTx] (0UL,0UL)
+        let (>>=) m f = Option.bind f m
+
+        let block =
+            "0000000000000000000000000000000000000000000000000000000000000000000000000000000" +
+            "10ee6ef1eb8bcf752290c0765c52e83a0cf72963773c3aa6f18524f97b4b55ee100000160e073fe" +
+            "8f20ffffff000000000000000000000000000000000000000327568a196fd2af61b99bd5578e80f" +
+            "44bb4b685973fd87f334623a503b5b67c65f54f0947eb311b6fdd36ccd5ab7b8fada7b55502abba" +
+            "816e8d65d83a26092ed9be653064be80f760b9d471dc9afbac2b24236c9f2eb0f08b7427942852d" +
+            "c780200000001000000000000000101eca101ba1e938c6a8cd10e031f2ac363f4176dcf4450e244" +
+            "2ebedb825fd33b1e000000000000000000000000000000000000000000000000000000000000000" +
+            "000000000000000000000000000000000000000000000000000000000000000000000000005f5e1" +
+            "000000000000"
+            |> FsBech32.Base16.decode
+            >>= Serialization.Block.deserialize
+            |> Option.get
 
         use client = ServiceBus.Client.create busName
 
@@ -178,7 +192,7 @@ let main argv =
         event.Set() |> ignore
     )
 
-    event.WaitOne() |> ignore    
+    event.WaitOne() |> ignore
 
     printfn "Closing..."
 
