src/Wallet.Tests/KeyPathParserTests.fs
@@ -1,0 +1,18 @@
+module KeyPathParserTests
+
+open NUnit.Framework
+open FsUnit
+open Wallet
+open ExtendedKey
+
+[<Test>]
+let ``can parse valid key path``() =
+    let path = KeyPathParser.parse "m/44'/258'/0'/0/0"
+
+    printfn "%A" path
+
+    let expected:Result<int list,string> = Ok [Hardened 44;Hardened 258;Hardened 0;0;0]
+
+    printfn "%A" expected
+
+    path |> should equal <| expected
