src/ContractExamples/Token.fst
@@ -32,8 +32,8 @@ let redeem txSkeleton contractHash returnAddress wallet =
 
   CR.ofOption "contract doesn't have enough zens to pay you" txSkeleton
 
-val main: txSkeleton -> hash -> string -> option data -> wallet:wallet -> cost (result (txSkeleton ** option message))  (2 + 66 + (64 + (64 + (64 + 64 + (Zen.Wallet.size wallet * 128 + 192) + 0)) + 25) + 29)
-let main txSkeleton contractHash command data wallet =
+val main: txSkeleton -> hash -> string -> sender -> option data -> wallet:wallet -> cost (result (txSkeleton ** option message))  (2 + 66 + (64 + (64 + (64 + 64 + (Zen.Wallet.size wallet * 128 + 192) + 0)) + 25) + 29)
+let main txSkeleton contractHash command sender data wallet =
   let! returnAddress = data >!> tryDict >?> tryFindLock "returnAddress" in
 
   match returnAddress with
@@ -48,5 +48,5 @@ let main txSkeleton contractHash command data wallet =
   | None ->
       ET.autoFailw "returnAddress is required"
 
-val cf: txSkeleton -> string -> option data -> wallet -> cost nat 24
-let cf _ _ _ wallet = ret  (2 + 66 + (64 + (64 + (64 + 64 + (Zen.Wallet.size wallet * 128 + 192) + 0)) + 25) + 29)
+val cf: txSkeleton -> string -> sender -> option data -> wallet -> cost nat 24
+let cf _ _ _ _ wallet = ret  (2 + 66 + (64 + (64 + (64 + 64 + (Zen.Wallet.size wallet * 128 + 192) + 0)) + 25) + 29)
